+++
title = "QCQI/演習 2.47"
author = ["Yasuhito Takamiya"]
date = 2021-04-20T00:00:00+09:00
draft = false
+++

\\(A\\) と \\(B\\) は[エルミート演算子]({{< relref "20210408114955-エルミート演算子" >}})だから、

\\[A^{\dagger} = A, B^{\dagger} = B\\]

ここで \\((i[A, B])^{\dagger}\\) を計算すると、

\begin{eqnarray\*}
(i[A, B])^{\dagger} &=& (i(AB - BA))^{\dagger} \\\\\\
  &=& (i(AB) - i(BA))^{\dagger}
\end{eqnarray\*}

[QCQI/演習 2.14]({{< relref "20210408102838-qcqi_演習_2_14" >}}) より、

\begin{eqnarray\*}
\phantom{(i[A, B])^{\dagger}} &=& i(BA)^{\dagger} - i(AB)^{\dagger} \\\\\\
  &=& iA^{\dagger}B^{\dagger}-iB^{\dagger}A^{\dagger} \\\\\\
  &=& iAB - iBA \\\\\\
  &=& i(AB - BA) \\\\\\
  &=& i[A, B]
\end{eqnarray\*}

よって \\((i[A, B])^{\dagger} = i[A,B]\\) なので、\\(i[A, B]\\) はエルミート演算子。
